src/program_proof/mvcc/wrbuf_sort_ents_by_key.v
@@ -1,0 +1,234 @@
+From Perennial.program_proof.mvcc Require Import
+     wrbuf_prelude wrbuf_repr
+     index_proof
+     tuple_repr tuple_own tuple_free tuple_write_lock.
+
+Section heap.
+Context `{!heapGS Σ, !mvcc_ghostG Σ}.
+
+(*****************************************************************)
+(* func swap(ents []WrEnt, i, j uint64)                          *)
+(*****************************************************************)
+Local Lemma wp_swap (entsS : Slice.t) (ents : list wrent) (i j : u64) :
+  {{{ slice.is_slice_small entsS (structTy WrEnt) 1 (wrent_to_val <$> ents) ∗
+      ⌜(int.nat i < length ents ∧ int.nat j < length ents)%nat⌝
+  }}}
+    swap (to_val entsS) #i #j
+  {{{ (ents' : list wrent), RET #();
+      slice.is_slice_small entsS (structTy WrEnt) 1 (wrent_to_val <$> ents') ∗
+      ⌜ents' ≡ₚ ents⌝
+  }}}.
+Proof.
+  iIntros (Φ) "[HentsS %Hbounds] HΦ".
+  destruct Hbounds as [Hi Hj].
+  apply list_lookup_lt in Hi as Hx.
+  destruct Hx as [x Hx].
+  apply list_lookup_lt in Hj as Hy.
+  destruct Hy as [y Hy].
+  iDestruct (is_slice_small_sz with "HentsS") as "%HentsLen".
+  rewrite fmap_length in HentsLen.
+  wp_call.
+  
+  (***********************************************************)
+  (* tmp := ents[i]                                          *)
+  (* ents[i] = ents[j]                                       *)
+  (* ents[j] = tmp                                           *)
+  (***********************************************************)
+  wp_apply (wp_SliceGet with "[$HentsS]").
+  { iPureIntro. by rewrite list_lookup_fmap Hx. }
+  iIntros "[HentsS %Htyx]".
+  wp_apply (wp_SliceGet with "[$HentsS]").
+  { iPureIntro. by rewrite list_lookup_fmap Hy. }
+  iIntros "[HentsS %Htyy]".
+  wp_apply (wp_SliceSet with "[$HentsS]").
+  { iPureIntro. split; last done. by rewrite list_lookup_fmap fmap_is_Some. }
+  iIntros "HentsS".
+  wp_apply (wp_SliceSet with "[$HentsS]").
+  { iPureIntro. split; last done.
+    rewrite -list_fmap_insert list_lookup_fmap fmap_is_Some.
+    apply lookup_lt_is_Some_2.
+    rewrite insert_length.
+    word.
+  }
+  iIntros "HentsS".
+  wp_pures.
+  iApply "HΦ".
+  iFrame.
+  do 2 rewrite -list_fmap_insert.
+  iFrame.
+  iPureIntro.
+  apply list_insert_insert_swap; done.
+Qed.
+
+(*********************************************************************)
+(* func (wrbuf *WrBuf) sortEntsByKey()                               *)
+(*********************************************************************)
+Theorem wp_wrbuf__sortEntsByKey wrbuf mods :
+  {{{ own_wrbuf_xtpls wrbuf mods }}}
+    WrBuf__sortEntsByKey #wrbuf
+  {{{ RET #(); own_wrbuf_xtpls wrbuf mods }}}.
+Proof.
+  iIntros (Φ) "Hwrbuf HΦ".
+  wp_call.
+  
+  (***********************************************************)
+  (* ents := wrbuf.ents                                      *)
+  (* var i uint64 = 1                                        *)
+  (***********************************************************)
+  iNamed "Hwrbuf".
+  wp_loadField.
+  wp_pures.
+  wp_apply (wp_ref_to); first by auto.
+  iIntros (iRef) "HiRef".
+  wp_pures.
+  iDestruct (is_slice_small_acc with "HentsS") as "[HentsS HentsC]".
+  iDestruct (is_slice_small_sz with "HentsS") as "%HentsLen".
+  rewrite fmap_length in HentsLen.
+
+  (***********************************************************)
+  (* for i < uint64(len(ents)) {                             *)
+  (*     var j uint64 = i                                    *)
+  (*     for j > 0 {                                         *)
+  (*         if ents[j - 1].key <= ents[j].key {             *)
+  (*             break                                       *)
+  (*         }                                               *)
+  (*         swap(ents, j - 1, j)                            *)
+  (*         j--                                             *)
+  (*     }                                                   *)
+  (*     i++                                                 *)
+  (* }                                                       *)
+  (***********************************************************)
+  set P := (λ (b : bool), ∃ (ents' : list wrent) (i : u64),
+               "HentsS" ∷ is_slice_small entsS (struct.t WrEnt) 1 (wrent_to_val <$> ents') ∗
+               "HiRef"  ∷ iRef ↦[uint64T] #i ∗
+               "%Hperm" ∷ ⌜ents' ≡ₚ ents⌝
+           )%I.
+  wp_apply (wp_forBreak_cond P with "[] [HentsS HiRef]").
+  { (* Outer loop body. *)
+    clear Φ.
+    iIntros (Φ) "!> HP HΦ".
+    iNamed "HP".
+    wp_load.
+    wp_apply (wp_slice_len).
+    wp_if_destruct; last first.
+    { (* Outer loop condition. *)
+      iApply "HΦ".
+      subst P. simpl.
+      eauto 10 with iFrame.
+    }
+    wp_load.
+    wp_apply (wp_ref_to); first by auto.
+    iIntros (jRef) "HjRef".
+    wp_pures.
+
+    (* Inner loop. *)
+    set Q := (λ (b : bool), ∃ (ents'' : list wrent) (j : u64),
+                "HentsS" ∷ is_slice_small entsS (struct.t WrEnt) 1 (wrent_to_val <$> ents'') ∗
+                "HjRef"  ∷ jRef ↦[uint64T] #j ∗
+                "%Hperm" ∷ ⌜ents'' ≡ₚ ents'⌝ ∗
+                "%Hle" ∷ ⌜int.Z j ≤ int.Z i⌝
+            )%I.
+    wp_apply (wp_forBreak_cond Q with "[] [HentsS HjRef]").
+    { (* Inner loop body. *)
+      clear Φ.
+      iIntros (Φ) "!> HQ HΦ".
+      iNamed "HQ".
+      wp_load.
+      wp_if_destruct; last first.
+      { (* Inner loop condition. *)
+        iApply "HΦ".
+        subst Q. simpl.
+        eauto 10 with iFrame.
+      }
+      wp_pures.
+
+      assert (Hboundj : (int.nat j < length ents'')%nat).
+      { apply Permutation_length in Hperm, Hperm0. word. }
+
+      (* Read key of entry at [j - 1]. *)
+      wp_load.
+      destruct (list_lookup_lt _ (wrent_to_val <$> ents'') (int.nat (word.sub j (U64 1)))) as [entx Hlookupx].
+      { rewrite fmap_length. word. }
+      wp_apply (wp_SliceGet with "[$HentsS]"); first done.
+      iIntros "[HentsS %Hty]".
+      wp_pures.
+      apply val_to_wrent_with_val_ty in Hty as (kx & vx & wx & tx & Hentx).
+      subst entx.
+      wp_pures.
+
+      (* Read key of entry at [j]. *)
+      wp_load.
+      destruct (list_lookup_lt _ (wrent_to_val <$> ents'') (int.nat j)) as [enty Hlookupy].
+      { rewrite fmap_length. word. }
+      wp_apply (wp_SliceGet with "[$HentsS]"); first done.
+      iIntros "[HentsS %Hty]".
+      wp_pures.
+      apply val_to_wrent_with_val_ty in Hty as (ky & vy & wy & ty & Henty).
+      subst enty.
+      wp_pures.
+
+      wp_if_destruct.
+      { (* Early return of inner loop. *)
+        iApply "HΦ". subst Q. simpl.
+        eauto with iFrame.
+      }
+      (* Swap entries at [j - 1] and at [j]. *)
+      do 2 wp_load.
+      wp_apply (wp_swap with "[$HentsS]").
+      { iPureIntro. word. }
+        
+      iIntros (ents1) "[HentsS %Hperm1]".
+      wp_load.
+      wp_store.
+      iApply "HΦ".
+      subst Q. simpl.
+      do 2 iExists _.
+      iFrame.
+      iPureIntro.
+      split; last by word.
+      by rewrite -Hperm0.
+    }
+    { (* Inner loop entry. *)
+      subst Q. simpl.
+      eauto with iFrame.
+    }
+    
+    (* Increment [i]. *)
+    iIntros "HQ".
+    subst Q. simpl.
+    iNamed "HQ".
+    wp_load.
+    wp_store.
+    iApply "HΦ".
+    subst P. simpl.
+    do 2 iExists _. iFrame.
+    iPureIntro.
+    by rewrite <- Hperm.
+  }
+  { (* Outer loop entry. *)
+    subst P. simpl.
+    eauto with iFrame.
+  }
+
+  (* RETURN. *)
+  iIntros "HP".
+  subst P. simpl.
+  iNamed "HP".
+  iDestruct ("HentsC" with "HentsS") as "HentsS".
+  wp_pures.
+  iApply "HΦ".
+  do 2 iExists _.
+  iFrame.
+  iPureIntro.
+  split.
+  { (* Prove [NoDup]. *)
+    by rewrite Hperm.
+  }
+  { (* Prove [list_to_map]. *)
+    rewrite Hmods.
+    apply list_to_map_proper; last by rewrite Hperm.
+    by apply NoDup_wrent_to_key_dbval.
+  }
+Qed.
+
+End heap.
